
\lesson{1}{22/4/23}{intro} 

\begin{itemize}
    \item First part: fundamental groups. We follow Munkres:
        \begin{itemize}
            \item Chap 9 `Fundamental group'
            \item Chap 11 `The Seifert-Van Kampen thm' and
            \item Chap 12/13 `Classification covering spaces'
        \end{itemize}
    \item Second part: Homology groups, via cudi, chapter of a book.
    \item 10 problems (solve them during the semester) No feedback during the semester, but asking questions is allowed. Working together is allowed.
    \item Exam (completely open book) First 4 questions: 1h30 prep. Last one 30 min, no prep
        \begin{enumerate}
            \item Theoretical question (open book, explain the proof, \ldots) \hfill /4
            \item New problem (comparable to one of the 10 problems)\hfill /4
            \item Explain your solution $n$-th problem solved at home \hfill /4
            \item Explain your solution $m$-th problem solved at home\hfill /4
            \item 4 small questions \hfill /4
        \end{enumerate}
        After the exam, hand in your solutions of the other problems. After a quick look, the points of 3.\ and 4.\ can be $\pm 1$ (in extreme cases $\pm 2$)
    \item No exercise classes for this course!
\end{itemize}

\setcounter{chapter}{-1}
\setcounter{chapter}{8}
\chapter{Fundamental group}

\setcounter{section}{50}
\section{Homotopy of paths}
\begin{definition}[Homotopy]
    Let $f,g:X\to Y$ be maps (so continuous). Then a homotopy between $f$ and $g$ is a continuous map $H: X\times I \to Y$ such that
    \begin{itemize}
        \item $H(x, 0) = f(x)$, $H(x, 1) = g(x)$ 
        \item For all $t \in I$, define $f_t: X \to  Y: x \mapsto  H(x, t)$
    \end{itemize}
    We say that $f$ is homotopic with $g$, we write $f \simeq g$.
    If $g$ is a constant map, we say that $f$ is null homotopic.
\end{definition}

\begin{definition}[Path homotopy]
    Let $f, g: I \to  X$ be two paths such that $f(0) = g(0) = x_0$ and $f(1) = g(1) = x_1$. Then $H: I \times  I \to  X$ is a path homotopy between $f$ and $g$, if and only if
    \begin{itemize}
        \item $H(s,0) = f(s)$ and  $H(s, 1) = g(s)$ (homotopy between maps)
        \item  $H(0, t) = x_0$ and $H(1, t) = x_1$ (start and end points fixed)
    \end{itemize}
    Notation: $f \simeq_p g$.
\end{definition}


\begin{lemma}
    $\simeq$ and  $\simeq_p$ are equivalence relations.
\end{lemma}
\begin{proof}
    \leavevmode
    \begin{itemize}
        \item Reflective: $F(x, t) = f(x)$
        \item Symmetric: $G(x, t) = H(x, 1-t)$ 
        \item Transitive:  Suppose $f \simeq g$ and  $g \simeq h$, with  $H_1, H_2$ resp.
            \[
                H(x, t) = \begin{cases}
                    H_1(x, 2t) & 0 \le t \le  \frac{1}{2}\\
                    H_2(x, 2t-1) & \frac{1}{2} \le  t \le  1
                \end{cases}
            . \qedhere
        \] 
    \end{itemize}
\end{proof}


\begin{eg}[Trivial, but important]
   Let $C \subset \R^n$ be a convex subset.
   \begin{itemize}
       \item Any two maps $f, g: X \to C$ are homotopic.
       \item Any two paths $f, g: I \to  C$ with $f(0) = g(0)$ and  $g(1) = f(1)$ are path homotopic.
   \end{itemize}

   Choose $H: X \times I \to  C: (x, t) \to  H(x, t) = (1-t) f(x) + t g(x)$.
\end{eg}


\subsection*{Product of paths}
Let $f: I\to X$, $g: I \to X$ be paths, $f(1) = g(0)$.
Define  \[
    f*g: I \to X: s \mapsto \begin{cases}
        f(2s) & 0 \le  s \le  \frac{1}{2}\\
        g(2s - 1) & \frac{1}{2}\le s\le 1.
\end{cases}
\]
\begin{remark}
    If $f$ is path homotopic to $f'$ and $g$ path homotopic to $g'$ (which means that $f(1) = f'(1) = g(0) = g'(0)$), then $f * g \simeq_p f' * g'$.
\end{remark}

So we can define $[f] * [g] := [f*g]$ with $[f] := \{g : I \to  X  \mid g \simeq_p f\} $

\begin{theorem}\leavevmode
    \begin{enumerate}
        \item $[f] * ([g] * [h])$  is defined iff $([f] * [g])*[h]$ is defined and in that case, they are equal.
        \item Let $e_x$ denote the constant path $e_x: I \to  X: s \mapsto x$, $x \in X$. If $f(0) = x_0$ and $f(1) = x_1$ then $[e_{x_0}] * [f] = [f]$ and $[f] * [e_{x_1}] = [f]$.
        \item Let $\overline{f} : I \to  X: s \mapsto  f(1-s)$. Then $[f] * [\overline{f}] = [e_{x_0}]$ and $[\overline{f}]*[f] = [e_{x_1}]$
    \end{enumerate}
\end{theorem}
\begin{proof}
    First, two observations
    \begin{itemize}
        \item Suppose $f\simeq_p g$ via homotopy $H$, $f, g: I\to X$.
            Let $k: X \to  Y$.
            Then $k  \circ  f \simeq_p k \circ g$ using $k  \circ H$.
        \item If $f*g$ (not necessarily path homotopic). Then $ k  \circ (f*g) = (k \circ f) * (k \circ g) .$ 
    \end{itemize}

    Now, the proof
    \begin{itemize}
        \item[2.]  Take $e_0: I \to  I: s \mapsto 0$.
            Take $i: I \to  I: s \mapsto s$ 
            Then $e_0*i$ is a path from $0$ to $1 \in I$.
            The path $i$ is also such a path.
            Because $I$ is a convex subset, $e_0*i$ and $i$ are path homotopic, $e_0 *i\simeq_p i$.
            Using one of our observations, we find that
            \begin{align*}
                f  \circ (e_0 * i) &\simeq_p  f  \circ i\\
                (f  \circ  e_0) * (f  \circ  i ) &\simeq_p f\\
                e_{x_0} * f  &\simeq_p f\\
                [e_{x_0}] * [f]  &= [f]
            .\end{align*}

        \item [3.] Note that $i * \overline{i} \simeq_p e_0$.
            Now, applying the same rules, we get 
            \begin{align*}
                f  \circ (i * \overline{i}) &\simeq_p f  \circ  e_0\\
                f * \overline{f} &\simeq_p  e_{x_0}\\
                [f] * [\overline{f}] & = [e_{x_0}]
            .\end{align*}
        \item[1.]  Remark: Only defined if $f(1) = g(0), g(1) = h(0)$.
            Note that $f*(g*h) \neq (f*g)*h$. The trajectory is the same, but the speed is not.

            Assume the product is defined.
            Suppose $[a, b]$,  $[c, d]$ are intervals in  $\R$.
            Then there is a unique positive (positive slope), linear map from $[a, b] \to [c,d]$.
            For any $a, b \in [0, 1)$ with $ 0<a<b<1$, we define a path
            \begin{align*}
                k_{a,b}: [0, 1] &\longrightarrow  X\\
                [0, a] & \xrightarrow{\text{lin.}}[0, 1] \xrightarrow{f}  X\\
                [a, b] & \xrightarrow{\text{lin.}}[0, 1] \xrightarrow{g}  X\\
                [b, 0] & \xrightarrow{\text{lin.}}[0, 1] \xrightarrow{h}  X\\
            \end{align*} 

            Then $f*(g*h) = k_{\frac{1}{2}, \frac{3}{4}}$ and $(f*g)*h = k_{\frac{1}{4}, \frac{1}{2}}$

            Let $\gamma$ be that path $\gamma:I \to  I$ with the following graphs:

            Note  that $\gamma \simeq_p i$.
            Now, using the fact that composition of positive linear maps is positive linear.
            \begin{align*}
                k_{c, d}  \circ  \gamma &\simeq_p  k_{c, d}  \circ i\\
                k_{a, b} &\simeq_p  k_{c, d},
            \end{align*} 
            which is what we wanted to show.
    \end{itemize}
\end{proof}


\section{Fundamental group}
\begin{definition}
    Let $X$ be a space and $x_0 \in X$, then the fundamental group of $X$ based at $x_0$ is
    \[
        \pi(X, x_0) = \{ [f]  \mid  f : I \to X, f(0) = f(1) = x_0\} 
    .\] 
    (Also $\pi_1(X, x_0)$ is used, first homotopy group of $X$ based at $x_0$)

    For $[f], [g] \in \pi(X, x_0)$, $[f] * [g]$ is always defined,  $[e_{x_0}]$ is an identity element, $*$ is associative and $[f]^{-1} = [\overline{f}]$. This makes $(\pi(X, x_0), *)$ a group.
\end{definition}
\begin{eg}
    If $C \subset \R^n$, convex then $\pi(X, x_0) = 1$.
    E.g. $\pi(B^2, x_0) = 1$.
\end{eg}

\begin{remark}
    All groups are a fundamental group of some space.
\end{remark}

Question: how does the group depend on  the base point?

\begin{theorem}[52.1]
    Let $X$ be a space, $x_0, x_1 \in X$ and $\alpha: I \to X$ a path from  $x_0$ to $x_1$.
    Then
    \begin{align*}
        \hat{\alpha}: \pi(X, x_0) &\longrightarrow\pi(x, x_1)\\
        [f] &\longmapsto  [\overline{\alpha}] * [f] * [\alpha]
    .\end{align*}
    is an isomorphisms of groups. Note however that this isomorphism depends on $\alpha$.
\end{theorem}
\begin{proof}
    Let $[f], [g] \in \pi_1(X, x_0)$.
    Then 
    \begin{align*}
        \hat{\alpha}([f]*[g]) &= [\overline{\alpha}] * [f] * [g] * [\alpha]\\
                              &= [\overline{\alpha}] *[f] * [\alpha] * [\overline{\alpha}] * [g] * [\alpha]\\
                              &= \hat{\alpha}[f] * \hat{\alpha}[g]
    .\end{align*}
    We can also construct the inverse, proving that these groups are isomorphic.
\end{proof}

\begin{remark}
    If $f: (x, x_0) \to (Y, y_0)$ is a map of pointed topology spaces ($f: X \to Y$ continuous and $f(x_0) = y_0$).
    Then \[
        f_*:\pi(X, x_0) \to  \pi(Y, y_0): [\gamma] \mapsto [f  \circ \gamma]
    \]
    is a morphism of groups, because of the two `rules' discussed previously, with
    \[
        (f \circ g)_* = f_*  \circ g_* \qquad (1_X)_* = 1_{\pi(X, x_0)}
    .\] 
\end{remark}
